Add interfaces around interop modules to avoid need for expose_interfaces from outside

src/arch/x64/interop/AESEncryptBE.fst
@@ -23,49 +23,10 @@ open Vale_aes128_encrypt_block_be
 
 assume val st_put (h:HS.mem) (p:HS.mem -> Type0) (f:(h0:HS.mem{p h0}) -> GTot HS.mem) : Stack unit (fun h0 -> p h0 /\ h == h0) (fun h0 _ h1 -> h == h0 /\ f h == h1)
 
-let b8 = B.buffer UInt8.t
+
 
 //The map from buffers to addresses in the heap, that remains abstract
 assume val addrs: addr_map
-
-let rec loc_locs_disjoint_rec (l:b8) (ls:list b8) : Type0 =
-  match ls with
-  | [] -> True
-  | h::t -> M.loc_disjoint (M.loc_buffer l) (M.loc_buffer h) /\ loc_locs_disjoint_rec l t
-
-let rec locs_disjoint_rec (ls:list b8) : Type0 =
-  match ls with
-  | [] -> True
-  | h::t -> loc_locs_disjoint_rec h t /\ locs_disjoint_rec t
-
-unfold
-let locs_disjoint (ls:list b8) : Type0 = normalize (locs_disjoint_rec ls)
-
-
-let keys_match (key:Ghost.erased (aes_key_LE AES_128)) (keys_b:B.buffer UInt8.t { B.length keys_b % 16 == 0 }) (h:HS.mem) =
-  let keys128_b = BV.mk_buffer_view keys_b Views.view128 in
-  let round_keys = key_to_round_keys_LE AES_128 (Ghost.reveal key) in
-  BV.as_seq h keys128_b == round_keys
-
-open FStar.Mul
-
-// TODO: Complete with your pre- and post-conditions
-let pre_cond (h:HS.mem) (output_b:b8) (input_b:b8) (key:Ghost.erased (aes_key_LE AES_128)) (keys_b:b8) =
-live h output_b /\ live h input_b /\ live h keys_b /\ locs_disjoint [output_b;input_b;keys_b] /\ length output_b % 16 == 0 /\ length input_b % 16 == 0 /\ length keys_b % 16 == 0 /\ B.length keys_b == (nr AES_128 + 1) * 16 /\
-  keys_match key keys_b h
-  /\ B.length output_b >= 1 /\ B.length input_b >= 1
-
-
-let post_cond (h0:HS.mem) (h1:HS.mem) (output_b:b8) (input_b:b8) (key:Ghost.erased (aes_key_LE AES_128)) (keys_b:b8) =
-  length input_b % 16 == 0 /\ length output_b % 16 == 0 /\ length keys_b % 16 == 0 /\
-    B.live h1 input_b /\ B.live h1 keys_b /\
-    M.modifies (M.loc_buffer output_b) h0 h1 /\
-    (let  input128_b = BV.mk_buffer_view  input_b Views.view128 in
-     let output128_b = BV.mk_buffer_view output_b Views.view128 in
-     BV.length input128_b >= 1 /\ BV.length output128_b >= 1 /\
-    (let  input_q = Seq.index (BV.as_seq h0 input128_b) 0 in 
-     let output_q = Seq.index (BV.as_seq h1 output128_b) 0 in
-     output_q == aes_encrypt_BE AES_128 (Ghost.reveal key) input_q))
 
 
 
@@ -108,9 +69,6 @@ let implies_post (va_s0:va_state) (va_sM:va_state) (va_fM:va_fuel) (output_b:b8)
   length_t_eq (TBase TUInt128) keys_b;
   ()
 
-val aes128_encrypt_block_be: output_b:b8 -> input_b:b8 -> key:Ghost.erased (aes_key_LE AES_128) -> keys_b:b8 -> Stack unit
-	(requires (fun h -> pre_cond h output_b input_b key keys_b ))
-	(ensures (fun h0 _ h1 -> post_cond h0 h1 output_b input_b key keys_b ))
 
 val ghost_aes128_encrypt_block_be: output_b:b8 -> input_b:b8 -> key:Ghost.erased (aes_key_LE AES_128) -> keys_b:b8 -> (h0:HS.mem{pre_cond h0 output_b input_b key keys_b }) -> GTot (h1:HS.mem{post_cond h0 h1 output_b input_b key keys_b })
 
