src/arch/x64/interop/GHash_extra.fst
@@ -33,92 +33,6 @@ let b8 = B.buffer UInt8.t
 //The map from buffers to addresses in the heap, that remains abstract
 assume val addrs: addr_map
 
-let rec loc_locs_disjoint_rec (l:b8) (ls:list b8) : Type0 =
-  match ls with
-  | [] -> True
-  | h::t -> M.loc_disjoint (M.loc_buffer l) (M.loc_buffer h) /\ loc_locs_disjoint_rec l t
-
-let rec locs_disjoint_rec (ls:list b8) : Type0 =
-  match ls with
-  | [] -> True
-  | h::t -> loc_locs_disjoint_rec h t /\ locs_disjoint_rec t
-
-unfold
-let locs_disjoint (ls:list b8) : Type0 = normalize (locs_disjoint_rec ls)
-
-let buffer_to_quad32 (b:B.buffer UInt8.t { B.length b % 16 == 0 /\ B.length b > 0 }) (h:HS.mem) : GTot quad32 =
-  let b128 = BV.mk_buffer_view b Views.view128 in
-  BV.as_buffer_mk_buffer_view b Views.view128;
-  BV.get_view_mk_buffer_view b Views.view128;
-  BV.length_eq b128;
-  assert (B.length b >= 16);
-  assert (BV.length b128 > 0);
-  BV.sel h b128 0
-
-let buffer_to_seq_quad32 (b:B.buffer UInt8.t { B.length b % 16 == 0 }) (h:HS.mem) : GTot (s:Seq.seq quad32 {Seq.length s == B.length b / 16} ) =
-  let b128 = BV.mk_buffer_view b Views.view128 in
-  BV.as_buffer_mk_buffer_view b Views.view128;
-  BV.get_view_mk_buffer_view b Views.view128;
-  BV.length_eq b128;
-  (BV.as_seq h b128)
-
-open FStar.Mul
-
-// TODO: Complete with your pre- and post-conditions
-let pre_cond (h:HS.mem) (in_b:b8) (hash_b:b8) (h_b:b8) (num_bytes:nat64) (orig_hash:Ghost.erased (quad32)) = live h in_b /\ live h hash_b /\ live h h_b /\ locs_disjoint [in_b;hash_b;h_b] /\ length in_b % 16 == 0 /\ length hash_b % 16 == 0 /\ length h_b % 16 == 0 /\
-   ( let mods = M.loc_buffer hash_b in 
-    B.live h in_b /\ B.live h hash_b /\ B.live h h_b /\ 
-    M.loc_disjoint (M.loc_buffer in_b) mods /\
-    M.loc_disjoint (M.loc_buffer h_b)  mods /\
-    
-    B.length in_b  == bytes_to_quad_size num_bytes * 16 /\
-    B.length in_b % 16 == 0 /\
-
-    B.length h_b == 16 /\
-    B.length hash_b == 16 /\
-
-    4096 * num_bytes < pow2_32 /\
-    256 * bytes_to_quad_size num_bytes < pow2_32 /\
-    
-    (let num_blocks = num_bytes / 16 in    
-     let old_hash = buffer_to_quad32 hash_b h in
-     //let new_hash = buffer_to_quad32 hash_b h' in
-     let h_val = buffer_to_quad32 h_b h in
-
-     // GHash reqs
-     let input = Seq.slice (buffer_to_seq_quad32 in_b h) 0 num_blocks in
-     old_hash == ghash_incremental0 h_val (Ghost.reveal orig_hash) input /\
-     
-     // Extra reqs
-     num_bytes % 16 <> 0 /\ 
-     0 < num_bytes /\ num_bytes < 16 * bytes_to_quad_size num_bytes /\
-     16 * (bytes_to_quad_size num_bytes - 1) < num_bytes /\
-
-     True
-    )
-)
-
-let post_cond (h:HS.mem) (h':HS.mem) (in_b:b8) (hash_b:b8) (h_b:b8) (num_bytes:nat64) (orig_hash:Ghost.erased (quad32)) = length in_b % 16 == 0 /\ length hash_b % 16 == 0 /\ length h_b % 16 == 0 /\
-    B.length in_b  == bytes_to_quad_size num_bytes * 16 /\
-    B.length h_b == 16 /\
-    B.length hash_b == 16 /\
-    (let mods = M.loc_buffer hash_b in
-    M.modifies mods h h' /\
-    B.live h in_b /\ B.live h hash_b /\ B.live h h_b /\
-    (let num_blocks = num_bytes / 16 in
-     let old_hash = buffer_to_quad32 hash_b h in
-     let new_hash = buffer_to_quad32 hash_b h' in
-     let h_val = buffer_to_quad32 h_b h in
-
-     let input_bytes = Seq.slice (le_seq_quad32_to_bytes (buffer_to_seq_quad32 in_b h')) 0 num_bytes in
-     let padded_bytes = pad_to_128_bits input_bytes in
-     let input_quads = le_bytes_to_seq_quad32 padded_bytes in
-     (num_bytes > 0 ==> Seq.length input_quads > 0 /\ 
-                       new_hash == ghash_incremental h_val (Ghost.reveal orig_hash) input_quads)
-    )
-  ) 
-
-
 //The initial registers and xmms
 assume val init_regs:reg -> nat64
 assume val init_xmms:xmm -> quad32
@@ -188,9 +102,6 @@ let implies_post (va_s0:va_state) (va_sM:va_state) (va_fM:va_fuel) (in_b:b8) (ha
   BV.as_seq_sel va_s0.mem.hs h128_b 0;
   ()
 
-val ghash_incremental_extra_stdcall: in_b:b8 -> hash_b:b8 -> h_b:b8 -> num_bytes:nat64 -> orig_hash:Ghost.erased (quad32) -> Stack unit
-	(requires (fun h -> pre_cond h in_b hash_b h_b num_bytes orig_hash ))
-	(ensures (fun h0 _ h1 -> post_cond h0 h1 in_b hash_b h_b num_bytes orig_hash ))
 
 val ghost_ghash_incremental_extra_stdcall: in_b:b8 -> hash_b:b8 -> h_b:b8 -> num_bytes:nat64 -> orig_hash:Ghost.erased (quad32) -> (h0:HS.mem{pre_cond h0 in_b hash_b h_b num_bytes orig_hash }) -> GTot (h1:HS.mem{post_cond h0 h1 in_b hash_b h_b num_bytes orig_hash })
 
@@ -229,4 +140,4 @@ let ghost_ghash_incremental_extra_stdcall in_b hash_b h_b num_bytes orig_hash h0
 
 let ghash_incremental_extra_stdcall in_b hash_b h_b num_bytes orig_hash  =
   let h0 = get() in
-  st_put h0 (fun h -> pre_cond h in_b hash_b h_b num_bytes orig_hash ) (ghost_ghash_incremental_extra_stdcall in_b hash_b h_b num_bytes orig_hash )
+  st_put h0 (fun h -> pre_cond h in_b hash_b h_b (UInt64.v num_bytes) orig_hash ) (ghost_ghash_incremental_extra_stdcall in_b hash_b h_b (UInt64.v num_bytes) orig_hash )
