src/arch/x64/interop/GHash_one_block.fst
@@ -27,55 +27,6 @@ let b8 = B.buffer UInt8.t
 //The map from buffers to addresses in the heap, that remains abstract
 assume val addrs: addr_map
 
-let rec loc_locs_disjoint_rec (l:b8) (ls:list b8) : Type0 =
-  match ls with
-  | [] -> True
-  | h::t -> M.loc_disjoint (M.loc_buffer l) (M.loc_buffer h) /\ loc_locs_disjoint_rec l t
-
-let rec locs_disjoint_rec (ls:list b8) : Type0 =
-  match ls with
-  | [] -> True
-  | h::t -> loc_locs_disjoint_rec h t /\ locs_disjoint_rec t
-
-unfold
-let locs_disjoint (ls:list b8) : Type0 = normalize (locs_disjoint_rec ls)
-
-open FStar.Mul
-
-
-let buffer_to_quad32 (b:B.buffer UInt8.t { B.length b % 16 == 0 /\ B.length b > 0 }) (h:HS.mem) : GTot quad32 =
-  let b128 = BV.mk_buffer_view b Views.view128 in
-  BV.as_buffer_mk_buffer_view b Views.view128;
-  BV.get_view_mk_buffer_view b Views.view128;
-  BV.length_eq b128;
-  assert (B.length b >= 16);
-  assert (BV.length b128 > 0);
-  BV.sel h b128 0
-  //index (BV.as_seq h b128) 0
-
-let buffer_to_seq_quad32 (b:B.buffer UInt8.t { B.length b % 16 == 0 }) (h:HS.mem) : GTot (s:Seq.seq quad32 {Seq.length s == B.length b / 16} ) =
-  let b128 = BV.mk_buffer_view b Views.view128 in
-  BV.as_buffer_mk_buffer_view b Views.view128;
-  BV.get_view_mk_buffer_view b Views.view128;
-  BV.length_eq b128;
-  (BV.as_seq h b128)
-
-// TODO: Complete with your pre- and post-conditions
-let pre_cond (h:HS.mem) (h_b:b8) (hash_b:b8) (input_b:b8) (offset:nat64) = live h h_b /\ live h hash_b /\ live h input_b /\ locs_disjoint [h_b;hash_b;input_b] /\ length h_b % 16 == 0 /\ length hash_b % 16 == 0 /\ length input_b % 16 == 0 /\
-  B.length h_b >= 16 /\ B.length hash_b >= 16 /\ B.length input_b >= 16 * (offset + 1)
-
-let post_cond (h:HS.mem) (h':HS.mem) (h_b:b8) (hash_b:b8) (input_b:b8) (offset:nat64) = length h_b % 16 == 0 /\ length hash_b % 16 == 0 /\ length input_b % 16 == 0 /\
- B.length h_b >= 16 /\ B.length hash_b >= 16 /\ B.length input_b >= 16 * (offset + 1) /\
-    M.modifies (M.loc_buffer hash_b) h h' /\
-    (let old_hash = buffer_to_quad32 hash_b h  in
-     let new_hash = buffer_to_quad32 hash_b h' in
-     let h_q      = buffer_to_quad32 h_b    h  in
-     let input    = buffer_to_seq_quad32 input_b h in
-     let input_quad = Seq.index input offset in
-     new_hash == ghash_incremental h_q old_hash (Seq.create 1 input_quad)
-    )
-  
-
 //The initial registers and xmms
 assume val init_regs:reg -> nat64
 assume val init_xmms:xmm -> quad32
@@ -126,10 +77,6 @@ let implies_post (va_s0:va_state) (va_sM:va_state) (va_fM:va_fuel) (h_b:b8) (has
   assert (Seq.equal (buffer_to_seq_quad32 input_b va_s0.mem.hs) (buffer128_as_seq (va_get_mem va_s0) input_b));  
   ()
 
-val ghash_incremental_one_block_buffer: h_b:b8 -> hash_b:b8 -> input_b:b8 -> offset:nat64 -> Stack unit
-	(requires (fun h -> pre_cond h h_b hash_b input_b offset ))
-	(ensures (fun h0 _ h1 -> post_cond h0 h1 h_b hash_b input_b offset ))
-
 val ghost_ghash_incremental_one_block_buffer: h_b:b8 -> hash_b:b8 -> input_b:b8 -> offset:nat64 -> (h0:HS.mem{pre_cond h0 h_b hash_b input_b offset }) -> GTot (h1:HS.mem{post_cond h0 h1 h_b hash_b input_b offset })
 
 let ghost_ghash_incremental_one_block_buffer h_b hash_b input_b offset h0 =
@@ -167,4 +114,4 @@ let ghost_ghash_incremental_one_block_buffer h_b hash_b input_b offset h0 =
 
 let ghash_incremental_one_block_buffer h_b hash_b input_b offset  =
   let h0 = get() in
-  st_put h0 (fun h -> pre_cond h h_b hash_b input_b offset ) (ghost_ghash_incremental_one_block_buffer h_b hash_b input_b offset )
+  st_put h0 (fun h -> pre_cond h h_b hash_b input_b (UInt64.v offset) ) (ghost_ghash_incremental_one_block_buffer h_b hash_b input_b (UInt64.v offset) )
