src/arch/x64/interop/Zero_quad32.fsti
@@ -1,0 +1,42 @@
+module Zero_quad32
+
+open LowStar.Buffer
+module B = LowStar.Buffer
+module BV = LowStar.BufferView
+open LowStar.Modifies
+module M = LowStar.Modifies
+open LowStar.ModifiesPat
+open FStar.HyperStack.ST
+module HS = FStar.HyperStack
+open Interop
+open Words_s
+open Types_s
+open X64.Machine_s
+open X64.Memory_i_s
+open X64.Vale.State_i
+open X64.Vale.Decls_i
+
+// TODO: Complete with your pre- and post-conditions
+let pre_cond (h:HS.mem) (b:b8) =    B.live h b /\
+    B.length b == 16
+
+
+let buffer_to_quad32 (b:B.buffer UInt8.t { B.length b % 16 == 0 /\ B.length b > 0 }) (h:HS.mem) : GTot quad32 =
+  let b128 = BV.mk_buffer_view b Views.view128 in
+  BV.as_buffer_mk_buffer_view b Views.view128;
+  BV.get_view_mk_buffer_view b Views.view128;
+  BV.length_eq b128;
+  assert (B.length b >= 16);
+  assert (BV.length b128 > 0);
+  BV.sel h b128 0
+
+
+let post_cond (h:HS.mem) (h':HS.mem) (b:b8) = length b == 16 /\
+    M.modifies (M.loc_buffer b) h h' /\
+    (let new_b = buffer_to_quad32 b h' in
+     new_b == Mkfour 0 0 0 0)
+
+noextract
+val zero_quad32_buffer: b:b8 -> Stack unit
+	(requires (fun h -> pre_cond h b ))
+	(ensures (fun h0 _ h1 -> post_cond h0 h1 b ))
